\documentclass{article}
\usepackage{amsmath, amssymb}

\begin{document}

\section*{Proof by Mathematical Induction}

We will prove that for all $n \in \mathbb{N}$,

\[
P(n): \sum_{k=1}^{n} k(k+1)(k+2) = \frac{n(n+1)(n+2)(n+3)}{4}
\]

\subsection*{Base Case: $n = 1$}

Left-hand side:
\[
\sum_{k=1}^{1} k(k+1)(k+2) = 1 \cdot 2 \cdot 3 = 6
\]

Right-hand side:
\[
\frac{1 \cdot 2 \cdot 3 \cdot 4}{4} = \frac{24}{4} = 6
\]

Therefore, $P(1)$ holds.

\subsection*{Inductive Hypothesis}

Assume that the formula holds for some $n \in \mathbb{N}$:

\[
\sum_{k=1}^{n} k(k+1)(k+2) = \frac{n(n+1)(n+2)(n+3)}{4}
\]

\subsection*{Inductive Step: Prove $P(n+1)$}

We want to show that:

\[
\sum_{k=1}^{n+1} k(k+1)(k+2) = \frac{(n+1)(n+2)(n+3)(n+4)}{4}
\]

Left-hand side:

\[
\sum_{k=1}^{n+1} k(k+1)(k+2) = \left( \sum_{k=1}^{n} k(k+1)(k+2) \right) + (n+1)(n+2)(n+3)
\]

Apply the inductive hypothesis:

\[
= \frac{n(n+1)(n+2)(n+3)}{4} + (n+1)(n+2)(n+3)
\]

Factor out $(n+1)(n+2)(n+3)$:

\[
= \left( \frac{n}{4} + 1 \right)(n+1)(n+2)(n+3) = \frac{n+4}{4}(n+1)(n+2)(n+3)
\]

\[
= \frac{(n+1)(n+2)(n+3)(n+4)}{4}
\]

This matches the right-hand side of $P(n+1)$. Therefore, $P(n+1)$ holds.

\subsection*{Conclusion}

By the principle of mathematical induction, the formula holds for all $n \in \mathbb{N}$.

\end{document}
